src/HOL/IMP/Abs_Int0_const.thy
@@ -1,0 +1,150 @@
+(* Author: Tobias Nipkow *)
+
+theory Abs_Int0_const
+imports Abs_Int0
+begin
+
+subsection "Constant Propagation"
+
+datatype cval = Const val | Any
+
+fun rep_cval where
+"rep_cval (Const n) = {n}" |
+"rep_cval (Any) = UNIV"
+
+fun plus_cval where
+"plus_cval (Const m) (Const n) = Const(m+n)" |
+"plus_cval _ _ = Any"
+
+lemma plus_cval_cases: "plus_cval a1 a2 =
+  (case (a1,a2) of (Const m, Const n) \<Rightarrow> Const(m+n) | _ \<Rightarrow> Any)"
+by(auto split: prod.split cval.split)
+
+instantiation cval :: SL_top
+begin
+
+fun le_cval where
+"_ \<sqsubseteq> Any = True" |
+"Const n \<sqsubseteq> Const m = (n=m)" |
+"Any \<sqsubseteq> Const _ = False"
+
+fun join_cval where
+"Const m \<squnion> Const n = (if n=m then Const m else Any)" |
+"_ \<squnion> _ = Any"
+
+definition "\<top> = Any"
+
+instance
+proof
+  case goal1 thus ?case by (cases x) simp_all
+next
+  case goal2 thus ?case by(cases z, cases y, cases x, simp_all)
+next
+  case goal3 thus ?case by(cases x, cases y, simp_all)
+next
+  case goal4 thus ?case by(cases y, cases x, simp_all)
+next
+  case goal5 thus ?case by(cases z, cases y, cases x, simp_all)
+next
+  case goal6 thus ?case by(simp add: Top_cval_def)
+qed
+
+end
+
+interpretation Rep rep_cval
+proof
+  case goal1 thus ?case
+    by(cases a, cases b, simp, simp, cases b, simp, simp)
+next
+  case goal2 show ?case by(simp add: Top_cval_def)
+qed
+
+interpretation Val_abs rep_cval Const plus_cval
+proof
+  case goal1 show ?case by simp
+next
+  case goal2 thus ?case
+    by(auto simp: plus_cval_cases split: cval.split)
+next
+  case goal3 thus ?case
+    by(auto simp: plus_cval_cases split: cval.split)
+qed
+
+text{* Could set the limit of the number of iterations to an arbitrarily
+large number because all ascending chains in this semilattice are finite. *}
+
+interpretation Abs_Int rep_cval Const plus_cval "(iter 15)"
+defines AI_const is AI
+and aval'_const is aval'
+and step_const is step
+proof qed (auto simp: iter_pfp strip_iter)
+
+text{* Straight line code: *}
+definition "test1_const =
+ ''y'' ::= N 7;
+ ''z'' ::= Plus (V ''y'') (N 2);
+ ''y'' ::= Plus (V ''x'') (N 0)"
+
+text{* Conditional: *}
+definition "test2_const =
+ IF Less (N 41) (V ''x'') THEN ''x'' ::= N 5 ELSE ''x'' ::= N 5"
+
+text{* Conditional, test is ignored: *}
+definition "test3_const =
+ ''x'' ::= N 42;
+ IF Less (N 41) (V ''x'') THEN ''x'' ::= N 5 ELSE ''x'' ::= N 6"
+
+text{* While: *}
+definition "test4_const =
+ ''x'' ::= N 0; WHILE B True DO ''x'' ::= N 0"
+
+text{* While, test is ignored: *}
+definition "test5_const =
+ ''x'' ::= N 0; WHILE Less (V ''x'') (N 1) DO ''x'' ::= N 1"
+
+text{* Iteration is needed: *}
+definition "test6_const =
+  ''x'' ::= N 0; ''y'' ::= N 0; ''z'' ::= N 2;
+  WHILE Less (V ''x'') (N 1) DO (''x'' ::= V ''y''; ''y'' ::= V ''z'')"
+
+text{* More iteration would be needed: *}
+definition "test7_const =
+  ''x'' ::= N 0; ''y'' ::= N 0; ''z'' ::= N 0; ''u'' ::= N 3;
+  WHILE Less (V ''x'') (N 1)
+  DO (''x'' ::= V ''y''; ''y'' ::= V ''z''; ''z'' ::= V ''u'')"
+
+text{* For readability: *}
+translations "x" <= "CONST V x"
+translations "x" <= "CONST N x"
+translations "x" <= "CONST Const x"
+translations "x < y" <= "CONST Less x y"
+translations "x" <= "CONST B x"
+translations "x" <= "CONST Up x"
+
+value [code] "show_acom (((step_const \<top>)^^0) (\<bottom>\<^sub>c test1_const))"
+value [code] "show_acom (((step_const \<top>)^^1) (\<bottom>\<^sub>c test1_const))"
+value [code] "show_acom (((step_const \<top>)^^2) (\<bottom>\<^sub>c test1_const))"
+value [code] "show_acom (((step_const \<top>)^^3) (\<bottom>\<^sub>c test1_const))"
+value [code] "show_acom (AI_const test1_const)"
+
+value [code] "show_acom (AI_const test2_const)"
+value [code] "show_acom (AI_const test3_const)"
+
+value [code] "show_acom (((step_const \<top>)^^0) (\<bottom>\<^sub>c test4_const))"
+value [code] "show_acom (((step_const \<top>)^^1) (\<bottom>\<^sub>c test4_const))"
+value [code] "show_acom (((step_const \<top>)^^2) (\<bottom>\<^sub>c test4_const))"
+value [code] "show_acom (((step_const \<top>)^^3) (\<bottom>\<^sub>c test4_const))"
+value [code] "show_acom (AI_const test4_const)"
+
+value [code] "show_acom (((step_const \<top>)^^0) (\<bottom>\<^sub>c test5_const))"
+value [code] "show_acom (((step_const \<top>)^^1) (\<bottom>\<^sub>c test5_const))"
+value [code] "show_acom (((step_const \<top>)^^2) (\<bottom>\<^sub>c test5_const))"
+value [code] "show_acom (((step_const \<top>)^^3) (\<bottom>\<^sub>c test5_const))"
+value [code] "show_acom (((step_const \<top>)^^4) (\<bottom>\<^sub>c test5_const))"
+value [code] "show_acom (((step_const \<top>)^^5) (\<bottom>\<^sub>c test5_const))"
+value [code] "show_acom (AI_const test5_const)"
+
+value [code] "show_acom (AI_const test6_const)"
+value [code] "show_acom (AI_const test7_const)"
+
+end
