src/HOL/IMP/Abs_Int0_fun.thy
@@ -1,0 +1,423 @@
+(* Author: Tobias Nipkow *)
+
+header "Abstract Interpretation"
+
+theory Abs_Int0_fun
+imports "~~/src/HOL/ex/Interpretation_with_Defs" Big_Step
+begin
+
+subsection "Annotated Commands"
+
+datatype 'a acom =
+  SKIP   'a                           ("SKIP {_}") |
+  Assign name aexp 'a                 ("(_ ::= _/ {_})" [1000, 61, 0] 61) |
+  Semi   "'a acom" "'a acom"          ("_;// _"  [60, 61] 60) |
+  If     bexp "'a acom" "'a acom" 'a
+    ("((IF _/ THEN _/ ELSE _)/ {_})"  [0, 0, 61, 0] 61) |
+  While  'a bexp "'a acom" 'a
+    ("({_}// WHILE _/ DO (_)// {_})"  [0, 0, 61, 0] 61)
+
+fun post :: "'a acom \<Rightarrow>'a" where
+"post (SKIP {P}) = P" |
+"post (x ::= e {P}) = P" |
+"post (c1; c2) = post c2" |
+"post (IF b THEN c1 ELSE c2 {P}) = P" |
+"post ({Inv} WHILE b DO c {P}) = P"
+
+fun strip :: "'a acom \<Rightarrow> com" where
+"strip (SKIP {a}) = com.SKIP" |
+"strip (x ::= e {a}) = (x ::= e)" |
+"strip (c1;c2) = (strip c1; strip c2)" |
+"strip (IF b THEN c1 ELSE c2 {a}) = (IF b THEN strip c1 ELSE strip c2)" |
+"strip ({a1} WHILE b DO c {a2}) = (WHILE b DO strip c)"
+
+fun anno :: "'a \<Rightarrow> com \<Rightarrow> 'a acom" where
+"anno a com.SKIP = SKIP {a}" |
+"anno a (x ::= e) = (x ::= e {a})" |
+"anno a (c1;c2) = (anno a c1; anno a c2)" |
+"anno a (IF b THEN c1 ELSE c2) =
+  (IF b THEN anno a c1 ELSE anno a c2 {a})" |
+"anno a (WHILE b DO c) =
+  ({a} WHILE b DO anno a c {a})"
+
+lemma strip_anno[simp]: "strip (anno a c) = c"
+by(induct c) simp_all
+
+fun map_acom :: "('a \<Rightarrow> 'b) \<Rightarrow> 'a acom \<Rightarrow> 'b acom" where
+"map_acom f (SKIP {a}) = SKIP {f a}" |
+"map_acom f (x ::= e {a}) = (x ::= e {f a})" |
+"map_acom f (c1;c2) = (map_acom f c1; map_acom f c2)" |
+"map_acom f (IF b THEN c1 ELSE c2 {a}) =
+  (IF b THEN map_acom f c1 ELSE map_acom f c2 {f a})" |
+"map_acom f ({a1} WHILE b DO c {a2}) =
+  ({f a1} WHILE b DO map_acom f c {f a2})"
+
+
+subsection "Orderings"
+
+class preord =
+fixes le :: "'a \<Rightarrow> 'a \<Rightarrow> bool" (infix "\<sqsubseteq>" 50)
+assumes le_refl[simp]: "x \<sqsubseteq> x"
+and le_trans: "x \<sqsubseteq> y \<Longrightarrow> y \<sqsubseteq> z \<Longrightarrow> x \<sqsubseteq> z"
+begin
+
+definition mono where "mono f = (\<forall>x y. x \<sqsubseteq> y \<longrightarrow> f x \<sqsubseteq> f y)"
+
+lemma monoD: "mono f \<Longrightarrow> x \<sqsubseteq> y \<Longrightarrow> f x \<sqsubseteq> f y" by(simp add: mono_def)
+
+lemma mono_comp: "mono f \<Longrightarrow> mono g \<Longrightarrow> mono (g o f)"
+by(simp add: mono_def)
+
+declare le_trans[trans]
+
+end
+
+text{* Note: no antisymmetry. Allows implementations where some abstract
+element is implemented by two different values @{prop "x \<noteq> y"}
+such that @{prop"x \<sqsubseteq> y"} and @{prop"y \<sqsubseteq> x"}. Antisymmetry is not
+needed because we never compare elements for equality but only for @{text"\<sqsubseteq>"}.
+*}
+
+class SL_top = preord +
+fixes join :: "'a \<Rightarrow> 'a \<Rightarrow> 'a" (infixl "\<squnion>" 65)
+fixes Top :: "'a" ("\<top>")
+assumes join_ge1 [simp]: "x \<sqsubseteq> x \<squnion> y"
+and join_ge2 [simp]: "y \<sqsubseteq> x \<squnion> y"
+and join_least: "x \<sqsubseteq> z \<Longrightarrow> y \<sqsubseteq> z \<Longrightarrow> x \<squnion> y \<sqsubseteq> z"
+and top[simp]: "x \<sqsubseteq> \<top>"
+begin
+
+lemma join_le_iff[simp]: "x \<squnion> y \<sqsubseteq> z \<longleftrightarrow> x \<sqsubseteq> z \<and> y \<sqsubseteq> z"
+by (metis join_ge1 join_ge2 join_least le_trans)
+
+lemma le_join_disj: "x \<sqsubseteq> y \<or> x \<sqsubseteq> z \<Longrightarrow> x \<sqsubseteq> y \<squnion> z"
+by (metis join_ge1 join_ge2 le_trans)
+
+end
+
+instantiation "fun" :: (type, SL_top) SL_top
+begin
+
+definition "f \<sqsubseteq> g = (ALL x. f x \<sqsubseteq> g x)"
+definition "f \<squnion> g = (\<lambda>x. f x \<squnion> g x)"
+definition "\<top> = (\<lambda>x. \<top>)"
+
+lemma join_apply[simp]: "(f \<squnion> g) x = f x \<squnion> g x"
+by (simp add: join_fun_def)
+
+instance
+proof
+  case goal2 thus ?case by (metis le_fun_def preord_class.le_trans)
+qed (simp_all add: le_fun_def Top_fun_def)
+
+end
+
+
+instantiation acom :: (preord) preord
+begin
+
+fun le_acom :: "('a::preord)acom \<Rightarrow> 'a acom \<Rightarrow> bool" where
+"le_acom (SKIP {S}) (SKIP {S'}) = (S \<sqsubseteq> S')" |
+"le_acom (x ::= e {S}) (x' ::= e' {S'}) = (x=x' \<and> e=e' \<and> S \<sqsubseteq> S')" |
+"le_acom (c1;c2) (c1';c2') = (le_acom c1 c1' \<and> le_acom c2 c2')" |
+"le_acom (IF b THEN c1 ELSE c2 {S}) (IF b' THEN c1' ELSE c2' {S'}) =
+  (b=b' \<and> le_acom c1 c1' \<and> le_acom c2 c2' \<and> S \<sqsubseteq> S')" |
+"le_acom ({Inv} WHILE b DO c {P}) ({Inv'} WHILE b' DO c' {P'}) =
+  (b=b' \<and> le_acom c c' \<and> Inv \<sqsubseteq> Inv' \<and> P \<sqsubseteq> P')" |
+"le_acom _ _ = False"
+
+lemma [simp]: "SKIP {S} \<sqsubseteq> c \<longleftrightarrow> (\<exists>S'. c = SKIP {S'} \<and> S \<sqsubseteq> S')"
+by (cases c) auto
+
+lemma [simp]: "x ::= e {S} \<sqsubseteq> c \<longleftrightarrow> (\<exists>S'. c = x ::= e {S'} \<and> S \<sqsubseteq> S')"
+by (cases c) auto
+
+lemma [simp]: "c1;c2 \<sqsubseteq> c \<longleftrightarrow> (\<exists>c1' c2'. c = c1';c2' \<and> c1 \<sqsubseteq> c1' \<and> c2 \<sqsubseteq> c2')"
+by (cases c) auto
+
+lemma [simp]: "IF b THEN c1 ELSE c2 {S} \<sqsubseteq> c \<longleftrightarrow>
+  (\<exists>c1' c2' S'. c = IF b THEN c1' ELSE c2' {S'} \<and> c1 \<sqsubseteq> c1' \<and> c2 \<sqsubseteq> c2' \<and> S \<sqsubseteq> S')"
+by (cases c) auto
+
+lemma [simp]: "{Inv} WHILE b DO c {P} \<sqsubseteq> w \<longleftrightarrow>
+  (\<exists>Inv' c' P'. w = {Inv'} WHILE b DO c' {P'} \<and> c \<sqsubseteq> c' \<and> Inv \<sqsubseteq> Inv' \<and> P \<sqsubseteq> P')"
+by (cases w) auto
+
+instance
+proof
+  case goal1 thus ?case by (induct x) auto
+next
+  case goal2 thus ?case
+  apply(induct x y arbitrary: z rule: le_acom.induct)
+  apply (auto intro: le_trans)
+  done
+qed
+
+end
+
+definition Top_acom :: "com \<Rightarrow> ('a::SL_top) acom" ("\<top>\<^sub>c") where
+"\<top>\<^sub>c = anno \<top>"
+
+lemma strip_Top_acom[simp]: "strip (\<top>\<^sub>c c) = c"
+by(simp add: Top_acom_def)
+
+lemma le_Top_acomp[simp]: "strip c' = c \<Longrightarrow> c' \<sqsubseteq> \<top>\<^sub>c c"
+by(induct c' arbitrary: c) (auto simp: Top_acom_def)
+
+
+subsubsection "Lifting"
+
+datatype 'a up = Bot | Up 'a
+
+instantiation up :: (SL_top)SL_top
+begin
+
+fun le_up where
+"Up x \<sqsubseteq> Up y = (x \<sqsubseteq> y)" |
+"Bot \<sqsubseteq> y = True" |
+"Up _ \<sqsubseteq> Bot = False"
+
+lemma [simp]: "(x \<sqsubseteq> Bot) = (x = Bot)"
+by (cases x) simp_all
+
+lemma [simp]: "(Up x \<sqsubseteq> u) = (\<exists>y. u = Up y & x \<sqsubseteq> y)"
+by (cases u) auto
+
+fun join_up where
+"Up x \<squnion> Up y = Up(x \<squnion> y)" |
+"Bot \<squnion> y = y" |
+"x \<squnion> Bot = x"
+
+lemma [simp]: "x \<squnion> Bot = x"
+by (cases x) simp_all
+
+definition "\<top> = Up \<top>"
+
+instance proof
+  case goal1 show ?case by(cases x, simp_all)
+next
+  case goal2 thus ?case
+    by(cases z, simp, cases y, simp, cases x, auto intro: le_trans)
+next
+  case goal3 thus ?case by(cases x, simp, cases y, simp_all)
+next
+  case goal4 thus ?case by(cases y, simp, cases x, simp_all)
+next
+  case goal5 thus ?case by(cases z, simp, cases y, simp, cases x, simp_all)
+next
+  case goal6 thus ?case by(cases x, simp_all add: Top_up_def)
+qed
+
+end
+
+definition bot_acom :: "com \<Rightarrow> ('a::SL_top)up acom" ("\<bottom>\<^sub>c") where
+"\<bottom>\<^sub>c = anno Bot"
+
+lemma strip_bot_acom[simp]: "strip(\<bottom>\<^sub>c c) = c"
+by(simp add: bot_acom_def)
+
+
+subsection "Absract Interpretation"
+
+text{* The representation of abstract by a set of concrete values: *}
+
+locale Rep =
+fixes rep :: "'a::SL_top \<Rightarrow> 'b set"
+assumes le_rep: "a \<sqsubseteq> b \<Longrightarrow> rep a \<subseteq> rep b"
+and rep_Top: "rep \<top> = UNIV"
+begin
+
+abbreviation in_rep (infix "<:" 50) where "x <: a == x : rep a"
+
+lemma in_rep_Top[simp]: "x <: \<top>"
+by(simp add: rep_Top)
+
+end
+
+definition rep_fun :: "('a \<Rightarrow> 'b set) \<Rightarrow> ('c \<Rightarrow> 'a) \<Rightarrow> ('c \<Rightarrow> 'b)set" where
+"rep_fun rep F = {f. \<forall>x. f x \<in> rep(F x)}"
+
+fun rep_up :: "('a \<Rightarrow> 'b set) \<Rightarrow> 'a up \<Rightarrow> 'b set" where
+"rep_up rep Bot = {}" |
+"rep_up rep (Up a) = rep a"
+
+text{* The interface for abstract values: *}
+
+(* FIXME: separate Rep interface needed? *)
+locale Val_abs = Rep rep for rep :: "'a::SL_top \<Rightarrow> val set" +
+fixes num' :: "val \<Rightarrow> 'a"
+and plus' :: "'a \<Rightarrow> 'a \<Rightarrow> 'a"
+assumes rep_num': "n <: num' n"
+and rep_plus': "n1 <: a1 \<Longrightarrow> n2 <: a2 \<Longrightarrow> n1+n2 <: plus' a1 a2"
+and mono_plus': "a1 \<sqsubseteq> b1 \<Longrightarrow> a2 \<sqsubseteq> b2 \<Longrightarrow> plus' a1 a2 \<sqsubseteq> plus' b1 b2"
+
+
+subsubsection "Post-fixed point iteration"
+
+fun iter :: "nat \<Rightarrow> (('a::SL_top) acom \<Rightarrow> 'a acom) \<Rightarrow> 'a acom \<Rightarrow> 'a acom" where
+"iter 0 f c = \<top>\<^sub>c (strip c)" |
+"iter (Suc n) f c = (let fc = f c in if fc \<sqsubseteq> c then c else iter n f fc)"
+(* code lemma?? *)
+
+lemma strip_iter: assumes "\<forall>c. strip(f c) = strip c"
+shows "strip(iter n f c) = strip c"
+apply (induction n arbitrary: c)
+ apply (metis iter.simps(1) strip_Top_acom)
+apply (simp add:Let_def)
+by (metis assms)
+
+lemma iter_pfp: assumes "\<forall>c. strip(f c) = strip c"
+shows "f(iter n f c) \<sqsubseteq> iter n f c"
+apply (induction n arbitrary: c)
+ apply(simp add: assms)
+apply (simp add:Let_def)
+done
+
+lemma iter_funpow: assumes "\<forall>c. strip(f c) = strip c"
+shows "iter n f x \<noteq> \<top>\<^sub>c (strip x) \<Longrightarrow> \<exists>k. iter n f x = (f^^k) x"
+apply(induction n arbitrary: x)
+ apply simp
+apply (auto simp: Let_def assms)
+ apply(metis funpow.simps(1) id_def)
+by (metis assms funpow.simps(2) funpow_swap1 o_apply)
+
+text{* For monotone @{text f}, @{term "iter f n x0"} yields the least
+post-fixed point above @{text x0}, unless it yields @{text Top}. *}
+
+lemma iter_least_pfp:
+assumes strip: "\<forall>c. strip(f c) = strip c"
+and mono: "\<And>x y. x \<sqsubseteq> y \<Longrightarrow> f x \<sqsubseteq> f y"
+and not_top: "iter n f x0 \<noteq> \<top>\<^sub>c (strip x0)"
+and "f p \<sqsubseteq> p" and "x0 \<sqsubseteq> p" shows "iter n f x0 \<sqsubseteq> p"
+proof-
+  obtain k where "iter n f x0 = (f^^k) x0"
+    using iter_funpow[OF strip not_top] by blast
+  moreover
+  { fix n have "(f^^n) x0 \<sqsubseteq> p"
+    proof(induction n)
+      case 0 show ?case by(simp add: `x0 \<sqsubseteq> p`)
+    next
+      case (Suc n) thus ?case
+        by (simp add: `x0 \<sqsubseteq> p`)(metis Suc `f p \<sqsubseteq> p` le_trans mono)
+    qed
+  } ultimately show ?thesis by simp
+qed
+
+type_synonym 'a st = "(name \<Rightarrow> 'a)"
+
+locale Abs_Int_Fun = Val_abs +
+fixes pfp :: "('a st up acom \<Rightarrow> 'a st up acom) \<Rightarrow> 'a st up acom \<Rightarrow> 'a st up acom"
+assumes pfp: "f(pfp f c) \<sqsubseteq> pfp f c"
+and strip_pfp: "\<forall>c. strip(f c) = strip c \<Longrightarrow> strip(pfp f c) = strip c"
+begin
+
+fun aval' :: "aexp \<Rightarrow> 'a st \<Rightarrow> 'a" where
+"aval' (N n) _ = num' n" |
+"aval' (V x) S = S x" |
+"aval' (Plus a1 a2) S = plus' (aval' a1 S) (aval' a2 S)"
+
+fun step :: "'a st up \<Rightarrow> 'a st up acom \<Rightarrow> 'a st up acom" where
+"step S (SKIP {P}) = (SKIP {S})" |
+"step S (x ::= e {P}) =
+  x ::= e {case S of Bot \<Rightarrow> Bot | Up S \<Rightarrow> Up(S(x := aval' e S))}" |
+"step S (c1; c2) = step S c1; step (post c1) c2" |
+"step S (IF b THEN c1 ELSE c2 {P}) =
+  (let c1' = step S c1; c2' = step S c2
+   in IF b THEN c1' ELSE c2' {post c1 \<squnion> post c2})" |
+"step S ({Inv} WHILE b DO c {P}) =
+  {S \<squnion> post c} WHILE b DO (step Inv c) {Inv}"
+
+lemma strip_step[simp]: "strip(step S c) = strip c"
+by(induct c arbitrary: S) (simp_all add: Let_def)
+
+
+definition AI :: "com \<Rightarrow> 'a st up acom" where
+"AI c = pfp (step \<top>) (\<bottom>\<^sub>c c)"
+
+
+abbreviation fun_in_rep :: "state \<Rightarrow> 'a st \<Rightarrow> bool" (infix "<:f" 50) where
+"s <:f S == s \<in> rep_fun rep S"
+
+notation fun_in_rep (infix "<:\<^sub>f" 50)
+
+lemma fun_in_rep_le: "s <:f S \<Longrightarrow> S \<sqsubseteq> T \<Longrightarrow> s <:f T"
+by(auto simp add: rep_fun_def le_fun_def dest: le_rep)
+
+abbreviation up_in_rep :: "state \<Rightarrow> 'a st up \<Rightarrow> bool"  (infix "<:up" 50) where
+"s <:up S == s : rep_up (rep_fun rep) S"
+
+notation (output) up_in_rep (infix "<:\<^sub>u\<^sub>p" 50)
+
+lemma up_fun_in_rep_le: "s <:up S \<Longrightarrow> S \<sqsubseteq> T \<Longrightarrow> s <:up T"
+by (cases S) (auto intro:fun_in_rep_le)
+
+lemma in_rep_Top_fun: "s <:f Top"
+by(simp add: Top_fun_def rep_fun_def)
+
+lemma in_rep_Top_up: "s <:up Top"
+by(simp add: Top_up_def in_rep_Top_fun)
+
+
+subsubsection "Monotonicity"
+
+lemma mono_aval': "S \<sqsubseteq> S' \<Longrightarrow> aval' e S \<sqsubseteq> aval' e S'"
+by(induction e)(auto simp: le_fun_def mono_plus')
+
+lemma mono_update: "a \<sqsubseteq> a' \<Longrightarrow> S \<sqsubseteq> S' \<Longrightarrow> S(x := a) \<sqsubseteq> S'(x := a')"
+by(simp add: le_fun_def)
+
+lemma step_mono: "S \<sqsubseteq> S' \<Longrightarrow> step S c \<sqsubseteq> step S' c"
+apply(induction c arbitrary: S S')
+apply (auto simp: Let_def mono_update mono_aval' le_join_disj split: up.split)
+done
+
+subsubsection "Soundness"
+
+lemma aval'_sound: "s <:f S \<Longrightarrow> aval a s <: aval' a S"
+by (induct a) (auto simp: rep_num' rep_plus' rep_fun_def)
+
+lemma in_rep_update: "\<lbrakk> s <:f S; i <: a \<rbrakk> \<Longrightarrow> s(x := i) <:f S(x := a)"
+by(simp add: rep_fun_def)
+
+lemma step_sound:
+  "step S c \<sqsubseteq> c \<Longrightarrow> (strip c,s) \<Rightarrow> t \<Longrightarrow> s <:up S \<Longrightarrow> t <:up post c"
+proof(induction c arbitrary: S s t)
+  case SKIP thus ?case
+    by simp (metis skipE up_fun_in_rep_le)
+next
+  case Assign thus ?case
+    apply (auto simp del: fun_upd_apply split: up.splits)
+    by (metis aval'_sound fun_in_rep_le in_rep_update)
+next
+  case Semi thus ?case by simp blast
+next
+  case (If b c1 c2 S0) thus ?case
+    apply(auto simp: Let_def)
+    apply (metis up_fun_in_rep_le)+
+    done
+next
+  case (While Inv b c P)
+  from While.prems have inv: "step Inv c \<sqsubseteq> c"
+    and "post c \<sqsubseteq> Inv" and "S \<sqsubseteq> Inv" and "Inv \<sqsubseteq> P" by(auto simp: Let_def)
+  { fix s t have "(WHILE b DO strip c,s) \<Rightarrow> t \<Longrightarrow> s <:up Inv \<Longrightarrow> t <:up Inv"
+    proof(induction "WHILE b DO strip c" s t rule: big_step_induct)
+      case WhileFalse thus ?case by simp
+    next
+      case (WhileTrue s1 s2 s3)
+      from WhileTrue.hyps(5)[OF up_fun_in_rep_le[OF While.IH[OF inv `(strip c, s1) \<Rightarrow> s2` `s1 <:up Inv`] `post c \<sqsubseteq> Inv`]]
+      show ?case .
+    qed
+  }
+  thus ?case using While.prems(2)
+    by simp (metis `s <:up S` `S \<sqsubseteq> Inv` `Inv \<sqsubseteq> P` up_fun_in_rep_le)
+qed
+
+lemma AI_sound: "(c,s) \<Rightarrow> t \<Longrightarrow> t <:up post(AI c)"
+by(auto simp: AI_def strip_pfp in_rep_Top_up intro: step_sound pfp)
+
+end
+
+text{* Problem: not executable because of the comparison of abstract states,
+i.e. functions, in the post-fixedpoint computation. *}
+
+end
