src/HOL/IMP/Abs_Int_Den/Abs_Int_den1_ivl.thy
@@ -1,0 +1,260 @@
+(* Author: Tobias Nipkow *)
+
+theory Abs_Int_den1_ivl
+imports Abs_Int_den1
+begin
+
+subsection "Interval Analysis"
+
+datatype ivl = I "int option" "int option"
+
+text{* We assume an important invariant: arithmetic operations are never
+applied to empty intervals @{term"I (Some i) (Some j)"} with @{term"j <
+i"}. This avoids special cases. Why can we assume this? Because an empty
+interval of values for a variable means that the current program point is
+unreachable. But this should actually translate into the bottom state, not a
+state where some variables have empty intervals. *}
+
+definition "rep_ivl i =
+ (case i of I (Some l) (Some h) \<Rightarrow> {l..h} | I (Some l) None \<Rightarrow> {l..}
+  | I None (Some h) \<Rightarrow> {..h} | I None None \<Rightarrow> UNIV)"
+
+definition "num_ivl n = I (Some n) (Some n)"
+
+instantiation option :: (plus)plus
+begin
+
+fun plus_option where
+"Some x + Some y = Some(x+y)" |
+"_ + _ = None"
+
+instance proof qed
+
+end
+
+definition empty where "empty = I (Some 1) (Some 0)"
+
+fun is_empty where
+"is_empty(I (Some l) (Some h)) = (h<l)" |
+"is_empty _ = False"
+
+lemma [simp]: "is_empty(I l h) =
+  (case l of Some l \<Rightarrow> (case h of Some h \<Rightarrow> h<l | None \<Rightarrow> False) | None \<Rightarrow> False)"
+by(auto split:option.split)
+
+lemma [simp]: "is_empty i \<Longrightarrow> rep_ivl i = {}"
+by(auto simp add: rep_ivl_def split: ivl.split option.split)
+
+definition "plus_ivl i1 i2 = ((*if is_empty i1 | is_empty i2 then empty else*)
+  case (i1,i2) of (I l1 h1, I l2 h2) \<Rightarrow> I (l1+l2) (h1+h2))"
+
+instantiation ivl :: SL_top
+begin
+
+definition le_option :: "bool \<Rightarrow> int option \<Rightarrow> int option \<Rightarrow> bool" where
+"le_option pos x y =
+ (case x of (Some i) \<Rightarrow> (case y of Some j \<Rightarrow> i\<le>j | None \<Rightarrow> pos)
+  | None \<Rightarrow> (case y of Some j \<Rightarrow> \<not>pos | None \<Rightarrow> True))"
+
+fun le_aux where
+"le_aux (I l1 h1) (I l2 h2) = (le_option False l2 l1 & le_option True h1 h2)"
+
+definition le_ivl where
+"i1 \<sqsubseteq> i2 =
+ (if is_empty i1 then True else
+  if is_empty i2 then False else le_aux i1 i2)"
+
+definition min_option :: "bool \<Rightarrow> int option \<Rightarrow> int option \<Rightarrow> int option" where
+"min_option pos o1 o2 = (if le_option pos o1 o2 then o1 else o2)"
+
+definition max_option :: "bool \<Rightarrow> int option \<Rightarrow> int option \<Rightarrow> int option" where
+"max_option pos o1 o2 = (if le_option pos o1 o2 then o2 else o1)"
+
+definition "i1 \<squnion> i2 =
+ (if is_empty i1 then i2 else if is_empty i2 then i1
+  else case (i1,i2) of (I l1 h1, I l2 h2) \<Rightarrow>
+          I (min_option False l1 l2) (max_option True h1 h2))"
+
+definition "Top = I None None"
+
+instance
+proof
+  case goal1 thus ?case
+    by(cases x, simp add: le_ivl_def le_option_def split: option.split)
+next
+  case goal2 thus ?case
+    by(cases x, cases y, cases z, auto simp: le_ivl_def le_option_def split: option.splits if_splits)
+next
+  case goal3 thus ?case
+    by(cases x, cases y, simp add: le_ivl_def join_ivl_def le_option_def min_option_def max_option_def split: option.splits)
+next
+  case goal4 thus ?case
+    by(cases x, cases y, simp add: le_ivl_def join_ivl_def le_option_def min_option_def max_option_def split: option.splits)
+next
+  case goal5 thus ?case
+    by(cases x, cases y, cases z, auto simp add: le_ivl_def join_ivl_def le_option_def min_option_def max_option_def split: option.splits if_splits)
+next
+  case goal6 thus ?case
+    by(cases x, simp add: Top_ivl_def le_ivl_def le_option_def split: option.split)
+qed
+
+end
+
+
+instantiation ivl :: L_top_bot
+begin
+
+definition "i1 \<sqinter> i2 = (if is_empty i1 \<or> is_empty i2 then empty else
+  case (i1,i2) of (I l1 h1, I l2 h2) \<Rightarrow>
+    I (max_option False l1 l2) (min_option True h1 h2))"
+
+definition "Bot = empty"
+
+instance
+proof
+  case goal1 thus ?case
+    by (simp add:meet_ivl_def empty_def meet_ivl_def le_ivl_def le_option_def max_option_def min_option_def split: ivl.splits option.splits)
+next
+  case goal2 thus ?case
+    by (simp add:meet_ivl_def empty_def meet_ivl_def le_ivl_def le_option_def max_option_def min_option_def split: ivl.splits option.splits)
+next
+  case goal3 thus ?case
+    by (cases x, cases y, cases z, auto simp add: le_ivl_def meet_ivl_def empty_def le_option_def max_option_def min_option_def split: option.splits if_splits)
+next
+  case goal4 show ?case by(cases x, simp add: Bot_ivl_def empty_def le_ivl_def)
+qed
+
+end
+
+instantiation option :: (minus)minus
+begin
+
+fun minus_option where
+"Some x - Some y = Some(x-y)" |
+"_ - _ = None"
+
+instance proof qed
+
+end
+
+definition "minus_ivl i1 i2 = ((*if is_empty i1 | is_empty i2 then empty else*)
+  case (i1,i2) of (I l1 h1, I l2 h2) \<Rightarrow> I (l1-h2) (h1-l2))"
+
+lemma rep_minus_ivl:
+  "n1 : rep_ivl i1 \<Longrightarrow> n2 : rep_ivl i2 \<Longrightarrow> n1-n2 : rep_ivl(minus_ivl i1 i2)"
+by(auto simp add: minus_ivl_def rep_ivl_def split: ivl.splits option.splits)
+
+
+definition "filter_plus_ivl i i1 i2 = ((*if is_empty i then empty else*)
+  i1 \<sqinter> minus_ivl i i2, i2 \<sqinter> minus_ivl i i1)"
+
+fun filter_less_ivl :: "bool \<Rightarrow> ivl \<Rightarrow> ivl \<Rightarrow> ivl * ivl" where
+"filter_less_ivl res (I l1 h1) (I l2 h2) =
+  ((*if is_empty(I l1 h1) \<or> is_empty(I l2 h2) then (empty, empty) else*)
+   if res
+   then (I l1 (min_option True h1 (h2 - Some 1)),
+         I (max_option False (l1 + Some 1) l2) h2)
+   else (I (max_option False l1 l2) h1, I l2 (min_option True h1 h2)))"
+
+interpretation Rep rep_ivl
+proof
+  case goal1 thus ?case
+    by(auto simp: rep_ivl_def le_ivl_def le_option_def split: ivl.split option.split if_splits)
+qed
+
+interpretation Val_abs rep_ivl num_ivl plus_ivl
+proof
+  case goal1 thus ?case by(simp add: rep_ivl_def num_ivl_def)
+next
+  case goal2 thus ?case
+    by(auto simp add: rep_ivl_def plus_ivl_def split: ivl.split option.splits)
+qed
+
+interpretation Rep1 rep_ivl
+proof
+  case goal1 thus ?case
+    by(auto simp add: rep_ivl_def meet_ivl_def empty_def min_option_def max_option_def split: ivl.split option.split)
+next
+  case goal2 show ?case by(auto simp add: Bot_ivl_def rep_ivl_def empty_def)
+qed
+
+interpretation
+  Val_abs1 rep_ivl num_ivl plus_ivl filter_plus_ivl filter_less_ivl
+proof
+  case goal1 thus ?case
+    by(auto simp add: filter_plus_ivl_def)
+      (metis rep_minus_ivl add_diff_cancel add_commute)+
+next
+  case goal2 thus ?case
+    by(cases a1, cases a2,
+      auto simp: rep_ivl_def min_option_def max_option_def le_option_def split: if_splits option.splits)
+qed
+
+interpretation
+  Abs_Int1 rep_ivl num_ivl plus_ivl filter_plus_ivl filter_less_ivl "(iter' 3)"
+defines afilter_ivl is afilter
+and bfilter_ivl is bfilter
+and AI_ivl is AI
+and aval_ivl is aval'
+proof qed (auto simp: iter'_pfp_above)
+
+
+fun list_up where
+"list_up bot = bot" |
+"list_up (Up x) = Up(list x)"
+
+value [code] "list_up(afilter_ivl (N 5) (I (Some 4) (Some 5)) Top)"
+value [code] "list_up(afilter_ivl (N 5) (I (Some 4) (Some 4)) Top)"
+value [code] "list_up(afilter_ivl (V ''x'') (I (Some 4) (Some 4))
+ (Up(FunDom(Top(''x'':=I (Some 5) (Some 6))) [''x''])))"
+value [code] "list_up(afilter_ivl (V ''x'') (I (Some 4) (Some 5))
+ (Up(FunDom(Top(''x'':=I (Some 5) (Some 6))) [''x''])))"
+value [code] "list_up(afilter_ivl (Plus (V ''x'') (V ''x'')) (I (Some 0) (Some 10))
+  (Up(FunDom(Top(''x'':= I (Some 0) (Some 100)))[''x''])))"
+value [code] "list_up(afilter_ivl (Plus (V ''x'') (N 7)) (I (Some 0) (Some 10))
+  (Up(FunDom(Top(''x'':= I (Some 0) (Some 100)))[''x''])))"
+
+value [code] "list_up(bfilter_ivl (Less (V ''x'') (V ''x'')) True
+  (Up(FunDom(Top(''x'':= I (Some 0) (Some 0)))[''x''])))"
+value [code] "list_up(bfilter_ivl (Less (V ''x'') (V ''x'')) True
+  (Up(FunDom(Top(''x'':= I (Some 0) (Some 2)))[''x''])))"
+value [code] "list_up(bfilter_ivl (Less (V ''x'') (Plus (N 10) (V ''y''))) True
+  (Up(FunDom(Top(''x'':= I (Some 15) (Some 20),''y'':= I (Some 5) (Some 7)))[''x'', ''y''])))"
+
+definition "test_ivl1 =
+ ''y'' ::= N 7;
+ IF Less (V ''x'') (V ''y'')
+ THEN ''y'' ::= Plus (V ''y'') (V ''x'')
+ ELSE ''x'' ::= Plus (V ''x'') (V ''y'')"
+value [code] "list_up(AI_ivl test_ivl1 Top)"
+
+value "list_up (AI_ivl test3_const Top)"
+
+value "list_up (AI_ivl test5_const Top)"
+
+value "list_up (AI_ivl test6_const Top)"
+
+definition "test2_ivl =
+ ''y'' ::= N 7;
+ WHILE Less (V ''x'') (N 100) DO ''y'' ::= Plus (V ''y'') (N 1)"
+value [code] "list_up(AI_ivl test2_ivl Top)"
+
+definition "test3_ivl =
+ ''x'' ::= N 0; ''y'' ::= N 100; ''z'' ::= Plus (V ''x'') (V ''y'');
+ WHILE Less (V ''x'') (N 11)
+ DO (''x'' ::= Plus (V ''x'') (N 1); ''y'' ::= Plus (V ''y'') (N -1))"
+value [code] "list_up(AI_ivl test3_ivl Top)"
+
+definition "test4_ivl =
+ ''x'' ::= N 0; ''y'' ::= N 0;
+ WHILE Less (V ''x'') (N 1001)
+ DO (''y'' ::= V ''x''; ''x'' ::= Plus (V ''x'') (N 1))"
+value [code] "list_up(AI_ivl test4_ivl Top)"
+
+text{* Nontermination not detected: *}
+definition "test5_ivl =
+ ''x'' ::= N 0;
+ WHILE Less (V ''x'') (N 1) DO ''x'' ::= Plus (V ''x'') (N -1)"
+value [code] "list_up(AI_ivl test5_ivl Top)"
+
+end
