src/HOL/IMP/Abs_Int_Den/Abs_Int_den2.thy
@@ -1,7 +1,7 @@
 (* Author: Tobias Nipkow *)
 
-theory Abs_Int2
-imports Abs_Int1_ivl
+theory Abs_Int_den2
+imports Abs_Int_den1_ivl
 begin
 
 context preord
