src/HOL/IMP/Abs_State.thy
@@ -1,0 +1,95 @@
+(* Author: Tobias Nipkow *)
+
+theory Abs_State
+imports Abs_Int0_fun
+  "~~/src/HOL/Library/Char_ord" "~~/src/HOL/Library/List_lexord"
+  (* Library import merely to allow string lists to be sorted for output *)
+begin
+
+subsection "Abstract State with Computable Ordering"
+
+text{* A concrete type of state with computable @{text"\<sqsubseteq>"}: *}
+
+datatype 'a st = FunDom "name \<Rightarrow> 'a" "name list"
+
+fun "fun" where "fun (FunDom f _) = f"
+fun dom where "dom (FunDom _ A) = A"
+
+definition [simp]: "inter_list xs ys = [x\<leftarrow>xs. x \<in> set ys]"
+
+definition "show_st S = [(x,fun S x). x \<leftarrow> sort(dom S)]"
+
+fun show_st_up where
+"show_st_up Bot = Bot" |
+"show_st_up (Up S) = Up(show_st S)"
+
+definition "show_acom = map_acom show_st_up"
+
+definition "lookup F x = (if x : set(dom F) then fun F x else \<top>)"
+
+definition "update F x y =
+  FunDom ((fun F)(x:=y)) (if x \<in> set(dom F) then dom F else x # dom F)"
+
+lemma lookup_update: "lookup (update S x y) = (lookup S)(x:=y)"
+by(rule ext)(auto simp: lookup_def update_def)
+
+definition "rep_st rep F = {f. \<forall>x. f x \<in> rep(lookup F x)}"
+
+instantiation st :: (SL_top) SL_top
+begin
+
+definition "le_st F G = (ALL x : set(dom G). lookup F x \<sqsubseteq> fun G x)"
+
+definition
+"join_st F G =
+ FunDom (\<lambda>x. fun F x \<squnion> fun G x) (inter_list (dom F) (dom G))"
+
+definition "\<top> = FunDom (\<lambda>x. \<top>) []"
+
+instance
+proof
+  case goal2 thus ?case
+    apply(auto simp: le_st_def)
+    by (metis lookup_def preord_class.le_trans top)
+qed (auto simp: le_st_def lookup_def join_st_def Top_st_def)
+
+end
+
+lemma mono_lookup: "F \<sqsubseteq> F' \<Longrightarrow> lookup F x \<sqsubseteq> lookup F' x"
+by(auto simp add: lookup_def le_st_def)
+
+lemma mono_update: "a \<sqsubseteq> a' \<Longrightarrow> S \<sqsubseteq> S' \<Longrightarrow> update S x a \<sqsubseteq> update S' x a'"
+by(auto simp add: le_st_def lookup_def update_def)
+
+context Rep
+begin
+
+abbreviation fun_in_rep :: "(name \<Rightarrow> 'b) \<Rightarrow> 'a st \<Rightarrow> bool" (infix "<:f" 50) where
+"s <:f S == s \<in> rep_st rep S"
+
+notation fun_in_rep (infix "<:\<^sub>f" 50)
+
+lemma fun_in_rep_le: "s <:f S \<Longrightarrow> S \<sqsubseteq> T \<Longrightarrow> s <:f T"
+apply(auto simp add: rep_st_def le_st_def dest: le_rep)
+by (metis in_rep_Top le_rep lookup_def subsetD)
+
+abbreviation in_rep_up :: "(name \<Rightarrow> 'b) \<Rightarrow> 'a st up \<Rightarrow> bool"  (infix "<:up" 50)
+where "s <:up S == s : rep_up (rep_st rep) S"
+
+notation (output) in_rep_up (infix "<:\<^sub>u\<^sub>p" 50)
+
+lemma up_fun_in_rep_le: "s <:up S \<Longrightarrow> S \<sqsubseteq> T \<Longrightarrow> s <:up T"
+by (cases S) (auto intro:fun_in_rep_le)
+
+lemma in_rep_up_iff: "x <:up u \<longleftrightarrow> (\<exists>u'. u = Up u' \<and> x <:f u')"
+by (cases u) auto
+
+lemma in_rep_Top_fun: "s <:f \<top>"
+by(simp add: rep_st_def lookup_def Top_st_def)
+
+lemma in_rep_Top_up: "s <:up \<top>"
+by(simp add: Top_up_def in_rep_Top_fun)
+
+end
+
+end
